bedrock2/src/Map/SortedListString.v
@@ -1,3 +1,2 @@
 Require bedrock2.Map.SortedList bedrock2.String.
-Definition map T : bedrock2.Map.map String.string T :=
-  SortedList.map (SortedList.parameters.Build_parameters _ T String.eqb String.ltb).
+Definition map T := SortedList.map (SortedList.parameters.Build_parameters _ T String.eqb String.ltb).
