bedrock2/src/Map/SortedListString_test.v
@@ -1,4 +1,4 @@
-Require Import bedrock2.Map Coq.Strings.String.
+Require Import coqutil.Map.Interface Coq.Strings.String.
 Require bedrock2.Map.SortedListString.
 Local Existing Instance bedrock2.Map.SortedListString.map.
 Local Open Scope string_scope. Local Open Scope list_scope.
@@ -12,5 +12,5 @@ Goal False.
   assert ((map.get (map.put (map.put (map.put map.empty "a" 6) "z" 0) "c" 9) "c") = Some 9) by exact eq_refl.
   assert ((map.get (map.put (map.put (map.put map.empty "a" 6) "z" 0) "c" 9) "z") = Some 0) by exact eq_refl.
   assert ((map.get (map.put (map.put (map.put map.empty "a" 6) "z" 0) "c" 9) "x") = None) by exact eq_refl.
-  assert (map.union (map.put (map.put map.empty "z" 7) "0" 0) (map.put (map.put (map.put map.empty "a" 6) "z" 0) "c" 9) = (map.put (map.put (map.put (map.put map.empty "a" 6) "z" 0) "c" 9) "0" 0)) by exact eq_refl.
+  assert (map.putmany (map.put (map.put map.empty "z" 7) "0" 0) (map.put (map.put (map.put map.empty "a" 6) "z" 0) "c" 9) = (map.put (map.put (map.put (map.put map.empty "a" 6) "z" 0) "c" 9) "0" 0)) by exact eq_refl.
 Abort.
