bedrock2/src/Notations.v
@@ -1,4 +1,4 @@
-Require Import bedrock2.Macros.
+Require Import coqutil.subst coqutil.unique.
 
 Notation "' x <- a | y ; f" :=
   (match a with
