bedrock2/src/Syntax.v
@@ -1,4 +1,4 @@
-Require Import bedrock2.Macros.
+Require Import coqutil.subst coqutil.unique.
 
 Require Import Coq.Numbers.BinNums.
   
