bedrock2/src/Tactics/rdelta.v
@@ -1,5 +1,0 @@
-Ltac rdelta x :=
-  match constr:(Set) with
-  | _ => let x := eval unfold x in x in x
-  | _ => x
-  end.
