bedrock2/src/Variables.v
@@ -1,4 +1,4 @@
-Require Import bedrock2.Macros bedrock2.Syntax.
+Require Import coqutil.subst coqutil.unique bedrock2.Syntax.
 
 Require Import Coq.Lists.List.
 
