bedrock2/src/Macros.v
@@ -1,8 +1,0 @@
-Notation "'subst!' y 'for' x 'in' f" := (match y with x => f end) (at level 10).
-
-Notation "'unique!' cls" := (ltac:(
-  match constr:(Set) with
-  | _ => let __ := constr:(_:cls) in fail 1 "unique!: already have an instance of" cls
-  | _ => exact cls%type
-  end))
-  (at level 10, only parsing).
